pure/Learn.Util.fst
@@ -14,3 +14,17 @@ let f_equal #a #b f x y = ()
 let prop_equal #a p x y = ()
 
 let assert_by p prf = prf ()
+
+
+module T = FStar.Tactics
+
+(* from F* tutorial *)
+let funext_on_eta (#a : Type) (#b: a -> Type) (f g : (x:a -> b x))
+                  (hp : (x:a -> Lemma (f x == g x)))
+  : squash (eta f == eta g)
+  = _ by T.(norm [delta_only [`%eta]];
+          pointwise (fun _ ->
+             try_with
+                     (fun _ -> mapply (quote hp))
+                     (fun _ -> trefl()));
+           trefl())
