pure/Learn.Util.fsti
@@ -18,14 +18,41 @@ val assert_by (p : Type) (prf : unit -> Lemma (ensures p)) : Lemma (ensures p)
 
 unfold let alias (#t : Type) (x : t) : Type = y:t{y == x}
 
-let cast (#a b : Type) (x : a) : Pure b (requires a == b) (ensures fun y -> y == x)
-  = x
-
-let cast_by (#a b : Type) (x : a) (pf : squash (a == b)) : Pure b (requires True) (ensures fun y -> y == x)
-  = x
-
 let iff_refl (a b : Type0) :
   Lemma (requires a == b) (ensures a <==> b)
   = ()
 
+
+unfold
+let cast (#a b : Type) (x : a) : Pure b (requires a == b) (ensures fun y -> y == x)
+  = x
+
+unfold
+let cast_by (#a b : Type) (x : a) (pf : squash (a == b)) : Pure b (requires True) (ensures fun y -> y == x)
+  = x
+
+
+irreducible let __util_func__ : unit = ()
+
+[@@ __util_func__]
+let const (a #b : Type) (y : b) (_ : a)
+  : b
+  = y
+
+[@@ __util_func__]
 let app_on (#a : Type) (x : a) (b : Type) (f : a -> b) = f x
+
+
+[@@ __util_func__]
+let eta (#a:Type) (#b: a -> Type) (f: (x:a -> b x)) = fun x -> f x
+
+val funext_on_eta (#a : Type) (#b: a -> Type) (f g : (x:a -> b x))
+                  (hp : (x:a -> Lemma (f x == g x)))
+  : squash (eta f == eta g)
+
+(* TODO? automatically discharge equalities with trefl : with_tactic ? *)
+let funext_eta (#a : Type) (#b : a -> Type) (f g : (x:a -> b x))
+               (ef : squash (f == eta f)) (eg : squash (g == eta g))
+               (eq : (x:a -> Lemma (f x == g x)))
+  : Lemma (f == g)
+  = funext_on_eta f g eq
