experiment/Experiment.Steel.Repr.Fun.fst
@@ -1,0 +1,743 @@
+module Experiment.Steel.Repr.Fun
+
+module U   = Learn.Util
+module L   = FStar.List.Pure
+module Ll  = Learn.List
+module Lf  = Learn.ListFun
+module Dl  = Learn.DList
+module ST  = Experiment.Steel.Repr.ST
+module Fin = FStar.Fin 
+
+open Experiment.Steel.Repr.ST
+
+type post_t (a : Type) = Lf.list_fun a Type
+unfold
+let post_ts (#a : Type) (post : post_t a) : a -> Dl.ty_list = post.lf_list
+type post_v (#a : Type) (post : post_t a) (x : a) = Dl.dlist (post_ts post x)
+type req_t = prop
+type ens_t (a : Type) (post : post_t a) = (x : a) -> post_v post x -> prop
+
+noeq
+type prog_tree : (a : Type u#a) -> (post : post_t u#a u#b a) -> Type u#(1 + max a b) =
+  | Tspec : (a : Type u#a) -> (post : post_t a) ->
+            (req : req_t) -> (ens : ens_t a post) ->
+            prog_tree a post
+  | Tret   : (a : Type u#a) -> (x : a) -> (post : post_t a) -> (sl : post_v post x) ->
+             prog_tree a post
+  | Tbind  : (a : Type u#a) -> (b : Type u#a) ->
+             (itm : post_t a) -> (post : post_t b) ->
+             (f : prog_tree a itm) -> (g : ((x : a) -> (sl : post_v itm x) -> prog_tree b post)) ->
+             prog_tree b post
+  | TbindP : (a : Type u#a) -> (b : Type u#a) ->
+             (post : post_t b) ->
+             (wp : pure_wp a) -> (x : unit -> PURE a wp) -> (g : a -> prog_tree b post) ->
+             prog_tree b post
+
+let rec tree_req (#a : Type) (#post : post_t a) (t : prog_tree a post)
+  : Tot req_t (decreases t)
+  = match t with
+  | Tspec _ _  req _ ->
+             req
+  | Tret _ _ _ _ ->
+             True
+  | Tbind a _  itm _  f g ->
+             tree_req f /\
+               (forall (x : a) (sl : post_v itm x) . tree_ens f x sl ==> tree_req (g x sl))
+  | TbindP a _  _  wp _ g ->
+             wp (fun (x : a) -> tree_req (g x)) /\ True
+
+and tree_ens (#a : Type) (#post : post_t a) (t : prog_tree a post)
+  : Tot (ens_t a post) (decreases t)
+  = match t with
+  | Tspec _ _  _ ens ->
+             ens
+  | Tret _ x  post0 sl ->
+             (fun x' (sl' : post_v post x') -> x' == x /\ sl' == sl)
+  | Tbind a _  itm post0  f g ->
+             (fun y (sl2 : post_v post y) -> tree_req f /\
+               (exists (x : a) (sl1 : post_v itm x) .
+                 tree_ens f x sl1 /\ tree_ens (g x sl1) y sl2))
+  | TbindP a _  post0  wp _ g ->
+             (fun y (sl1 : post_v post y) -> as_requires wp /\
+               (exists (x : a) . as_ensures wp x /\ tree_ens (g x) y sl1))
+
+
+(*** Repr.ST --> Repr.Fun *)
+
+module T = FStar.Tactics
+open FStar.Calc
+open Learn.Logic
+
+#push-options "--fuel 1 --ifuel 1"
+
+type post_src (pre_n : nat) (post_n : nat) = Fin.fin post_n -> option (Fin.fin pre_n)
+
+let post_src_of_shape (#pre_n : nat) (#post_n : nat) (s : ST.shape_tree pre_n post_n)
+  : Tot (post_src pre_n post_n)
+  = match s with
+  | Sequiv n p ->
+           (fun i -> Some (p i))
+  | Sspec  pre_n post_n frame_n ->
+           (fun i -> if i < post_n then None else Some (i - post_n + pre_n))
+  | Sret   n ->
+           (fun i -> None)
+  | Sbind  pre_n itm_n post_n f g ->
+            // bind returns all the selectors because with the current hypothesis, we need a value of the bound
+            // type in order to prove that the propagated value (through g and f) has the correct type
+           (fun i -> None)
+  | SbindP pre_n post_n g ->
+           (fun i -> None)
+
+let post_src_ty
+      (#a : Type) (#pre : ST.pre_t) (#post : ST.post_t a) (t : ST.prog_tree a pre post)
+      (s : ST.prog_shape t) (i : Fin.fin post.lf_len) (x : a)
+  : Lemma (requires Some? (post_src_of_shape s i))
+          (ensures  Lf.lf_index post i x == L.index pre (Some?.v (post_src_of_shape s i)))
+  = match t with
+    | ST.Tequiv _ _ _ -> ()
+    | ST.Tspec  _ pre post frame _ _ ->
+             Ll.append_index pre frame (i - post.lf_len + (L.length pre));
+             Ll.append_index (post.lf_list x) frame i
+    | ST.Tret _ _ _ | ST.Tbind _ _  _ _ _  _ _ | ST.TbindP _ _  _ _  _ _ _ -> ()
+
+noeq
+type post_bij_t' (#pre_n : nat) (#post_n : nat) (s : post_src pre_n post_n) = {
+  post'_n : nat;
+  post'_f : (i : Fin.fin post_n {None? (s i)}) -> Fin.fin post'_n;
+  post'_g : Fin.fin post'_n -> (i : Fin.fin post_n  {None? (s i)});
+}
+
+type post_bij_t (#pre_n : nat) (#post_n : nat) (s : post_src pre_n post_n) =
+  r : post_bij_t' s {
+    (forall (i : Fin.fin post_n {None? (s i)}) . {:pattern (r.post'_g (r.post'_f i))}
+      r.post'_g (r.post'_f i) = i) /\
+    (forall (j : Fin.fin r.post'_n) . {:pattern (r.post'_f (r.post'_g j))}
+      r.post'_f (r.post'_g j) = j)
+  }
+
+let rec mk_post_bij (#pre_n : nat) (#post_n : nat) (s : post_src pre_n post_n)
+  : Tot (post_bij_t s) (decreases post_n)
+  = if post_n = 0 then {
+       post'_n = 0;
+       post'_f = (fun _ -> false_elim ());
+       post'_g = (fun _ -> false_elim ())}
+    else
+      let s' : post_src pre_n (post_n - 1) = fun i -> s (i+1) in
+      let p' = mk_post_bij s' in
+      match s 0 with
+      | Some _ -> { post'_n = p'.post'_n;
+                   post'_f = (fun i -> p'.post'_f (i-1));
+                   post'_g = (fun j -> p'.post'_g j + 1)}
+      | None   -> { post'_n = p'.post'_n + 1;
+                   post'_f = (fun i -> if i = 0 then 0 else (p'.post'_f (i-1) + 1));
+                   post'_g = (fun j -> if j = 0 then 0 else (p'.post'_g (j-1) + 1))}
+
+let post_bij (#post_n : nat) (#pre_n : nat) (s : ST.shape_tree pre_n post_n)
+  : Tot (post_bij_t (post_src_of_shape s))
+  = match s with
+  | Sequiv n p ->
+           { post'_n = 0; post'_f = (fun _ -> false_elim ()); post'_g = (fun _ -> false_elim ()) }
+  | Sspec  pre_n post_n frame_n ->
+           { post'_n = post_n;
+             post'_f = (fun (i : Fin.fin (post_n + frame_n) {None? (post_src_of_shape s i)}) -> i);
+             post'_g = (fun j -> j) }
+  | Sret   n ->
+           { post'_n = n; post'_f = (fun i -> i); post'_g = (fun j -> j) }
+  | Sbind  pre_n itm_n post_n f g ->
+           { post'_n = post_n; post'_f = (fun i -> i); post'_g = (fun j -> j) }
+  | SbindP pre_n post_n g ->
+           { post'_n = post_n; post'_f = (fun i -> i); post'_g = (fun j -> j) }
+
+let post_Fun_of_ST
+      (#a : Type u#a) (post : ST.post_t u#a u#b a)
+      (#pre_n : nat) (s : ST.shape_tree pre_n post.lf_len)
+  : post_t u#a u#b a
+  = let p' = post_bij s in
+    { lf_len  = p'.post'_n;
+      lf_list = fun (x : a) -> Ll.initi 0 p'.post'_n (fun i -> L.index (post.lf_list x) (p'.post'_g i)) }
+
+// TODO? define with post : ty_list
+let sel_Fun_of_ST
+      (#a : Type u#a) (#pre_n : nat) (post : ST.post_t u#a u#b a)
+      (s : ST.shape_tree pre_n post.lf_len)
+      (x : a) (post_val : Dl.dlist (ST.post_ts post x))
+  : post_v (post_Fun_of_ST post s) x
+  = let p' = post_bij s in
+    Dl.initi 0 p'.post'_n _ (fun i -> Dl.index post_val (p'.post'_g i))
+
+unfold
+let return_Fun_post'_of_ST
+      (#a : Type u#a) (#pre_n : nat) (post : ST.post_t u#a u#b a)
+      (s : ST.shape_tree pre_n post.lf_len)
+      (x : a) (post_val : Dl.dlist (ST.post_ts post x))
+  : prog_tree a (post_Fun_of_ST post s)
+  = Tret a x (post_Fun_of_ST post s) (sel_Fun_of_ST post s x post_val)
+
+// TODO? remove the dependency in [t]
+let sel_ST_of_Fun
+      (#a : Type) (#pre : ST.pre_t) (#post : ST.post_t a) (t : ST.prog_tree a pre post)
+      (s : ST.prog_shape t)
+      (sl0 : Dl.dlist pre) (x : a) (sl1' : post_v (post_Fun_of_ST post s) x)
+  : Dl.dlist (ST.post_ts post x)
+  =
+    let p' = post_bij s in
+    Dl.initi_ty (ST.post_ts post x)
+             (fun i -> match post_src_of_shape s i with
+                    | Some j -> (**) post_src_ty t s i x;
+                               U.cast (L.index (ST.post_ts post x) i)
+                                      (Dl.index sl0 j)
+                    | None   -> U.cast (L.index (ST.post_ts post x) i)
+                                      (Dl.index sl1' (p'.post'_f i)))
+
+#push-options "--z3rlimit 20"
+let sel_Fun_ST_Fun
+      (#a : Type) (#pre : ST.pre_t) (#post : ST.post_t a) (t : ST.prog_tree a pre post)
+      (s : ST.prog_shape t)
+      (sl0 : Dl.dlist pre) (x : a) (sl1' : post_v (post_Fun_of_ST post s) x)
+  : Lemma (sel_Fun_of_ST post s x (sel_ST_of_Fun t s sl0 x sl1') == sl1')
+  = Dl.dlist_extensionality
+         (sel_Fun_of_ST post s x (sel_ST_of_Fun t s sl0 x sl1')) sl1'
+    begin fun i ->
+      let p' = post_bij s in
+      let post_ST = sel_ST_of_Fun t s sl0 x sl1' in
+      calc (==) {
+        Dl.index (sel_Fun_of_ST post s x post_ST) i;
+      == {}
+        U.cast (L.index (post_ts (post_Fun_of_ST post s) x) i)
+          (Dl.index post_ST ((post_bij s).post'_g i));
+      == {}
+        Dl.index sl1' ((post_bij s).post'_f ((post_bij s).post'_g i));
+      == {}
+        Dl.index sl1' i;
+      }
+   end
+#pop-options
+
+
+let post_Fun_of_ST__spec
+      (#a : Type) (post : ST.post_t a) (frame : ST.post_t a)
+      (pre_n : nat)
+  : Lemma (ensures post_Fun_of_ST (append_post_t post frame) (Sspec pre_n post.lf_len frame.lf_len)
+                == Lf.eta post)
+  =
+    let post' = post_Fun_of_ST (append_post_t post frame) (Sspec pre_n post.lf_len frame.lf_len) in
+    Lf.lf_eta_extensionality post' (Lf.eta post)
+         (assert (post' == Lf.eta post') by T.(trefl ())) (_ by T.(trefl ()))
+         (fun x i -> Ll.append_index (post.lf_list x) (frame.lf_list x) i)
+
+let post_Fun_of_ST__ret
+      (#a : Type) (post : ST.post_t a)
+  : Lemma (ensures post_Fun_of_ST post (Sret post.lf_len) == Lf.eta post)
+  =
+    let post' = post_Fun_of_ST post (Sret post.lf_len) in
+    Lf.lf_eta_extensionality post' (Lf.eta post)
+         (assert (post' == Lf.eta post') by T.(trefl ())) (_ by T.(trefl ()))
+         (fun x i -> ())
+
+
+(* TODO? markers *)
+let rec repr_Fun_of_ST
+          (#a : Type u#a) (#pre : ST.pre_t u#b) (#post : ST.post_t u#a u#b a)
+          (t : ST.prog_tree a pre post)
+  : Tot ((s : ST.prog_shape t) -> Dl.dlist pre -> prog_tree a (post_Fun_of_ST post s))
+        (decreases t)
+  = ST.match_prog_tree t
+      (fun a pre post t -> (s : ST.prog_shape t) -> Dl.dlist pre ->
+         prog_tree a (post_Fun_of_ST post s))
+    begin fun (*ST.Tequiv*) pre post0 p -> fun s sl0 ->
+            Tret unit' Unit' (Lf.const unit' []) Dl.DNil
+    end
+    begin fun (*ST.Tspec*) a pre post frame req ens -> fun s sl0' ->
+            (**) post_Fun_of_ST__spec post (post_t_of_ts a frame) (L.length pre);
+            (**) let post'  = post_Fun_of_ST (append_post_t post (post_t_of_ts a frame)) s in
+            let sl0 : Dl.dlist pre = (Dl.splitAt_ty pre frame sl0')._1 in
+            Tspec a (Lf.eta post) (req sl0) (ens sl0) <: prog_tree a post'
+    end
+    begin fun (*ST.Tret*) a x post -> fun s sl ->
+            (**) post_Fun_of_ST__ret post;
+            U.cast (prog_tree a (post_Fun_of_ST post s)) (Tret a x (Lf.eta post) sl)
+    end
+    begin fun (*ST.Tbind*) a b pre itm post f g -> fun s sl0 ->
+            (**) let Sbind _ _ _ s_f s_g = s in
+            Tbind a b  _ _ (repr_Fun_of_ST f s_f sl0) (fun x sl1' ->
+            let sl1 = sel_ST_of_Fun f s_f sl0 x sl1' in
+            Tbind b b  (post_Fun_of_ST post #(L.length (ST.post_ts itm x)) s_g) _
+                       (repr_Fun_of_ST (g x) s_g sl1) (fun y sl2' ->
+            let sl2 = sel_ST_of_Fun (g x) s_g sl1 y sl2' in
+            return_Fun_post'_of_ST post s y sl2))
+    end
+    begin fun (*ST.TbindP*) a b pre post wp f g -> fun s sl0 ->
+            (**) let SbindP _ _ s_g = s in
+            TbindP a b _ wp f (fun x ->
+            Tbind  b b (post_Fun_of_ST post #(L.length #Type pre) s_g) _
+                       (repr_Fun_of_ST (g x) s_g sl0) (fun y sl1' ->
+            let sl1 = sel_ST_of_Fun (g x) s_g sl0 y sl1' in
+            return_Fun_post'_of_ST post s y sl1))
+    end
+    
+#pop-options
+
+(*
+irreducible let print_util (#a : Type) (x : a) : prop = True
+
+let test (#a : Type u#a) (#pre : ST.pre_t u#b) (#post : ST.post_t u#a u#b a)
+          (t : ST.prog_tree a pre post)
+          (s : ST.prog_struct (L.length pre) post.lf_len {ST.prog_tree_struct t s})
+          (sl0 : Dl.dlist pre)
+  = assert (print_util (repr_Fun_of_ST t s sl0))
+      by T.(norm [delta_only [`%repr_Fun_of_ST]; zeta]; qed ())
+*)
+
+(***** soundness of ST --> Fun *)
+
+#push-options "--fuel 1 --ifuel 0"
+
+let post_eq_src (#pre #post : Dl.ty_list) (sl0 : Dl.dlist pre) (sl1 : Dl.dlist post)
+                (s : post_src (L.length pre) (L.length post))
+  : prop
+  = forall (i : Fin.fin (L.length post)) .
+      Some? (s i) ==> Dl.index sl1 i === Dl.index sl0 (Some?.v (s i))
+
+let sel_ST_of_Fun_eq_src
+      #a #pre #post (t : ST.prog_tree a pre post) (s : ST.prog_shape t)
+      (sl0 : Dl.dlist pre) (x : a) (sl1' : post_v (post_Fun_of_ST post s) x)
+  : Lemma (post_eq_src sl0 (sel_ST_of_Fun t s sl0 x sl1') (post_src_of_shape s))
+  = introduce forall (i : Fin.fin post.lf_len) .
+      Some? (post_src_of_shape s i) ==>
+      Dl.index (sel_ST_of_Fun t s sl0 x sl1') i === Dl.index sl0 (Some?.v (post_src_of_shape s i))
+    with introduce _ ==> _
+    with _ . post_src_ty t s i x
+
+#push-options "--z3rlimit 20"
+let post_eq_src_ST_Fun_ST
+      #a #pre #post  (t : ST.prog_tree a pre post) (s : ST.prog_shape t)
+      (sl0 : Dl.dlist pre) (x : a) (sl1 : Dl.dlist (ST.post_ts post x))
+  : Lemma (requires post_eq_src sl0 sl1 (post_src_of_shape s))
+          (ensures  sel_ST_of_Fun t s sl0 x (sel_Fun_of_ST post s x sl1) == sl1)
+  =
+    Dl.dlist_extensionality (sel_ST_of_Fun t s sl0 x (sel_Fun_of_ST post s x sl1)) sl1
+    begin fun i ->
+      match post_src_of_shape s i with
+      | Some j -> post_src_ty t s i x;
+                 calc (==) {
+                   Dl.index (sel_ST_of_Fun t s sl0 x (sel_Fun_of_ST post s x sl1)) i;
+                 == {}
+                   U.cast (L.index (ST.post_ts post x) i) (Dl.index sl0 j);
+                 == {(*by [post_eq_src] *)}
+                   Dl.index sl1 i;
+                 }
+      | None -> ()
+    end
+#pop-options
+
+(* TODO? def de post_eq_src *)
+let post_eq_src_iff
+      #a #pre #post (t : ST.prog_tree a pre post) (s : ST.prog_shape t)
+      (sl0 : Dl.dlist pre) (x : a) (sl1 : Dl.dlist (ST.post_ts post x))
+  : Lemma (post_eq_src sl0 sl1 (post_src_of_shape s)
+           <==> sl1 == sel_ST_of_Fun t s sl0 x (sel_Fun_of_ST post s x sl1))
+  = sel_ST_of_Fun_eq_src t s sl0 x (sel_Fun_of_ST post s x sl1);
+    FStar.Classical.move_requires (post_eq_src_ST_Fun_ST t s sl0 x) sl1
+
+
+unfold
+let req_equiv #a #pre #post (t : ST.prog_tree a pre post) (s : ST.prog_shape t)
+      (sl0 : Dl.dlist pre)
+  : prop
+  = ST.tree_req t sl0 <==> tree_req (repr_Fun_of_ST t s sl0)
+
+unfold
+let ens_equiv #a #pre #post (t : ST.prog_tree a pre post) (s : ST.prog_shape t)
+      (sl0 : Dl.dlist pre) (res : a) (sl1 : Dl.dlist (ST.post_ts post res))
+  : prop
+  = ST.tree_ens t sl0 res sl1 <==>
+   (post_eq_src sl0 sl1 (post_src_of_shape s) /\
+    tree_ens (repr_Fun_of_ST t s sl0) res (sel_Fun_of_ST post s res sl1))
+
+let ens_equiv_rev #a #pre #post (t : ST.prog_tree a pre post) (s : ST.prog_shape t)
+      (sl0 : Dl.dlist pre) (res : a) (sl1' : post_v (post_Fun_of_ST post s) res)
+  : Lemma (requires ens_equiv t s sl0 res (sel_ST_of_Fun t s sl0 res sl1'))
+          (ensures  ST.tree_ens t sl0 res (sel_ST_of_Fun t s sl0 res sl1') <==>
+                    tree_ens (repr_Fun_of_ST t s sl0) res sl1')
+  =
+    sel_ST_of_Fun_eq_src t s sl0 res sl1';
+    sel_Fun_ST_Fun t s sl0 res sl1'
+
+#push-options "--z3rlimit 10"
+let repr_Fun_of_ST_ens__Tspec a pre post frame req ens s sl0 x sl1
+  : Lemma (ensures ens_equiv (ST.Tspec a pre post frame req ens) s sl0 x sl1)
+  =
+    post_Fun_of_ST__spec post (post_t_of_ts a frame) (L.length pre);
+    let sl0', frame0 = Dl.splitAt_ty pre frame sl0 in
+    let sl1', frame1 = Dl.splitAt_ty (ST.post_ts post x) frame sl1 in
+
+    Dl.splitAt_ty_append pre frame sl0;
+    Dl.splitAt_ty_append (ST.post_ts post x) frame sl1;
+
+    Dl.dlist_extensionality
+      (sel_Fun_of_ST (append_post_t post (post_t_of_ts a frame)) s x sl1) sl1'
+      (fun i -> Dl.append_index sl1' frame1 i);
+    
+    introduce frame1 == frame0 ==>
+            (forall (i : int {post.lf_len <= i /\ i < post.lf_len + L.length frame}) .
+                Dl.index sl1 i === Dl.index sl0 (i - post.lf_len + L.length pre))
+      with _ . introduce forall (i : int {post.lf_len <= i /\ i < post.lf_len + L.length frame}) .
+                   Dl.(index (append sl1' frame1)) i ===
+                   Dl.(index (append sl0' frame0)) (i - post.lf_len + L.length pre)
+      with (Dl.append_index sl1' frame1 i;
+            Dl.append_index sl0' frame0 (i - post.lf_len + L.length pre));
+
+    introduce (forall (i : int {post.lf_len <= i /\ i < post.lf_len + L.length frame}) .
+                Dl.index sl1 i === Dl.index sl0 (i - post.lf_len + L.length pre))
+            ==> frame1 == frame0
+      with _ . Dl.dlist_extensionality frame1 frame0 (fun i ->
+        eliminate forall (i : int {post.lf_len <= i /\ i < post.lf_len + L.length frame}) .
+                  Dl.index sl1 i === Dl.index sl0 (i - post.lf_len + L.length pre)
+          with (i + post.lf_len);
+        Dl.append_index sl1' frame1 (i + post.lf_len);
+        Dl.append_index sl0' frame0 (i + L.length pre))
+#pop-options
+
+#push-options "--z3rlimit 20"
+let repr_Fun_of_ST_req__Tbind a b pre (itm : ST.post_t a) post
+      f (g : (x : a) -> ST.prog_tree b (ST.post_ts itm x) post)
+      (s_f  : prog_shape f)
+      (s_g : ST.shape_tree itm.lf_len post.lf_len {forall (x : a) . ST.prog_has_shape (g x) s_g})
+      sl0
+      (pre_eq_g  : (x : a) -> (sl1 : Dl.dlist (ST.post_ts itm x)) ->
+                   Lemma (req_equiv (g x) s_g sl1))
+      (post_eq_f : (x : a) -> (sl1 : Dl.dlist (ST.post_ts itm x)) ->
+                   Lemma (requires ST.tree_req f sl0) (ensures ens_equiv f s_f sl0 x sl1))
+  : Lemma
+      (requires ST.tree_req f sl0 <==> tree_req (repr_Fun_of_ST f s_f sl0))
+      (ensures  req_equiv (ST.Tbind a b pre itm post f g) (Sbind _ _ _ s_f s_g) sl0)
+  =
+    let t = ST.Tbind a b pre itm post f g in
+    let s = Sbind _ _ _ s_f s_g in
+    let r_f = repr_Fun_of_ST f s_f sl0 in
+    let r_g (x : a) (sl1 : Dl.dlist (ST.post_ts itm x)) = repr_Fun_of_ST (g x) s_g sl1 in
+    let itm' = post_Fun_of_ST itm s_f in
+
+    assert (req_equiv t s sl0 == (
+      (ST.tree_req f sl0 /\
+      (forall (x : a) (sl1 : Dl.dlist (ST.post_ts itm x)) .
+        ST.tree_ens f sl0 x sl1 ==> ST.tree_req (g x) sl1))
+    <==>
+      (tree_req r_f /\
+      (forall (x : a) (sl1' : post_v itm' x) .
+        tree_ens r_f x sl1' ==>
+      (let sl1 = sel_ST_of_Fun f s_f sl0 x sl1' in
+        tree_req (r_g x sl1) /\
+      (forall (y : b) (sl2' : post_v (post_Fun_of_ST post #(L.length (post_ts itm x)) s_g) y) .
+        tree_ens (r_g x sl1) y sl2' ==> True))))
+    )) by T.(trefl ());
+
+    introduce forall (x : a) . ST.tree_req f sl0 ==> (
+      (forall (sl1 : Dl.dlist (ST.post_ts itm x)) . ST.tree_ens f sl0 x sl1 ==> ST.tree_req (g x) sl1) <==>
+      (forall (sl1' : post_v itm' x) .
+        tree_ens r_f x sl1' ==>
+        tree_req (r_g x (sel_ST_of_Fun f s_f sl0 x sl1'))))
+      with introduce _ ==> _
+      with _ . begin
+        introduce forall (sl1 : Dl.dlist (ST.post_ts itm x)) . ens_equiv f s_f sl0 x sl1
+          with post_eq_f x sl1;
+        FStar.Classical.forall_intro (post_eq_src_iff f s_f sl0 x);
+        forall_morph_iff #(post_v itm' x)
+          (fun sl1' -> ST.tree_ens f sl0 x (sel_ST_of_Fun f s_f sl0 x sl1') ==>
+                    ST.tree_req (g x) (sel_ST_of_Fun f s_f sl0 x sl1'))
+          (fun sl1' -> tree_ens r_f x sl1' ==>
+                    tree_req (r_g x (sel_ST_of_Fun f s_f sl0 x sl1')))
+          (fun sl1' -> ens_equiv_rev f s_f sl0 x sl1';
+                    pre_eq_g x (sel_ST_of_Fun f s_f sl0 x sl1'))
+      end
+#pop-options
+
+#push-options "--z3rlimit 60"
+let repr_Fun_of_ST_ens__Tbind a b pre (itm : ST.post_t a) post
+      f (g : (x : a) -> ST.prog_tree b (ST.post_ts itm x) post)
+      (s_f  : prog_shape f)
+      (s_g : ST.shape_tree itm.lf_len post.lf_len {forall (x : a) . ST.prog_has_shape (g x) s_g})
+      sl0 y sl2
+      (pre_eq_g  : (x : a) -> (sl1 : Dl.dlist (ST.post_ts itm x)) ->
+                   Lemma (req_equiv (g x) s_g sl1))
+      (post_eq_f : (x : a) -> (sl1 : Dl.dlist (ST.post_ts itm x)) ->
+                   Lemma (ens_equiv f s_f sl0 x sl1))
+      (post_eq_g : (x : a) -> (sl1 : Dl.dlist (ST.post_ts itm x)) ->
+                   Lemma (requires ST.tree_req (g x) sl1) (ensures ens_equiv (g x) s_g sl1 y sl2))
+  : Lemma
+      (requires ST.tree_req (ST.Tbind a b pre itm post f g) sl0 /\
+                tree_req (repr_Fun_of_ST f s_f sl0))
+      (ensures  ens_equiv (ST.Tbind a b pre itm post f g) (Sbind _ _ _ s_f s_g) sl0 y sl2)
+  =
+    let t = ST.Tbind a b pre itm post f g in
+    let s = Sbind _ _ _ s_f s_g in
+    let r_f   = repr_Fun_of_ST f s_f sl0 in
+    let itm'  = post_Fun_of_ST itm s_f in
+    let r_g (x : a) (sl1 : Dl.dlist (ST.post_ts itm x)) = repr_Fun_of_ST (g x) s_g sl1 in
+    let post'g = post_Fun_of_ST post s_g in
+    let post'  = post_Fun_of_ST post s in
+    let sl2' : post_v post' y = sel_Fun_of_ST post s y sl2 in
+
+    assert (ens_equiv t s sl0 y sl2 ==
+      (ST.tree_req f sl0 /\
+       (exists (x : a) (sl1 : Dl.dlist (ST.post_ts itm x)) .
+         ST.tree_ens f sl0 x sl1 /\ ST.tree_ens (g x) sl1 y sl2)
+     <==>
+      (post_eq_src sl0 sl2 (post_src_of_shape s) /\
+      (tree_req r_f /\
+       (exists (x : a) (sl1' : post_v itm' x) .
+         tree_ens r_f x sl1' /\
+       (let sl1 = sel_ST_of_Fun f s_f sl0 x sl1' in
+        let r_g = r_g x sl1 in
+         tree_req r_g /\
+        (exists (yg : b) (sl2g : post_v (post_Fun_of_ST post #(L.length (post_ts itm x)) s_g) yg) .
+         tree_ens r_g yg sl2g /\
+        (let sl2f : Dl.dlist (post_ts post yg) = sel_ST_of_Fun (g x) s_g sl1 yg sl2g in
+         tree_ens (Tret b yg post' (sel_Fun_of_ST post s yg sl2f)) y sl2'
+         ))))))
+    )) by T.(trefl ());
+    
+    assert (ST.tree_req f sl0);
+    assert (post_eq_src sl0 sl2 (post_src_of_shape s));
+
+    introduce forall (x : a) .
+       (exists (sl1 : Dl.dlist (ST.post_ts itm x)) . ST.tree_ens f sl0 x sl1 /\ ST.tree_ens (g x) sl1 y sl2)
+    <==> (exists (sl1' : post_v itm' x) .
+         tree_ens r_f x sl1' /\
+       (let sl1 = sel_ST_of_Fun f s_f sl0 x sl1' in
+        let r_g = r_g x sl1 in
+         tree_req r_g /\
+        (exists (sl2g : post_v post'g y) .
+         tree_ens r_g y sl2g /\
+         sl2' == sel_Fun_of_ST post s y (sel_ST_of_Fun (g x) s_g sl1 y sl2g)
+         )))
+    with begin
+      introduce forall (sl2g : post_v post'g y) (sl1 : Dl.dlist (ST.post_ts itm x)) .
+        sl2' == sel_Fun_of_ST post s y (sel_ST_of_Fun (g x) s_g sl1 y sl2g)
+        <==> (sl2g == sel_Fun_of_ST post s_g y sl2 /\
+           post_eq_src sl1 sl2 (post_src_of_shape s_g))
+      with begin
+        let sl2gST = sel_ST_of_Fun (g x) s_g sl1 y sl2g in
+        // [sel_Fun_of_ST post s y] is injective (for s = [Sbind _]), the inverse is sel_ST_of_Fun
+        U.assert_by (sel_Fun_of_ST post s y sl2 == sel_Fun_of_ST post s y sl2gST
+                  ==> sl2 == sl2gST)
+          (fun () -> post_eq_src_ST_Fun_ST t s sl0 y sl2;
+                     post_eq_src_ST_Fun_ST t s sl0 y sl2gST);
+        sel_Fun_ST_Fun (g x) s_g sl1 y sl2g;
+        post_eq_src_iff (g x) s_g sl1 y sl2
+      end;
+
+      FStar.Classical.forall_intro (post_eq_f x);
+      FStar.Classical.forall_intro (post_eq_src_iff f s_f sl0 x);
+
+      exists_morph_iff #(post_v itm' x)
+        (fun sl1' -> ST.tree_ens f sl0 x (sel_ST_of_Fun f s_f sl0 x sl1') /\
+                  ST.tree_ens (g x) (sel_ST_of_Fun f s_f sl0 x sl1') y sl2)
+        (fun sl1' -> tree_ens r_f x sl1' /\
+                 (let sl1 = sel_ST_of_Fun f s_f sl0 x sl1' in
+                  let r_g = r_g x sl1 in
+                  tree_req r_g /\
+                  post_eq_src sl1 sl2 (post_src_of_shape s_g) /\
+                  tree_ens r_g y (sel_Fun_of_ST post s_g y sl2)))
+        (fun sl1' ->
+          let sl1 = sel_ST_of_Fun f s_f sl0 x sl1' in
+          post_eq_f x sl1;
+          ens_equiv_rev f s_f sl0 x sl1';
+          pre_eq_g x sl1;
+          FStar.Classical.move_requires (post_eq_g x) sl1
+        )
+    end
+#pop-options
+
+let repr_Fun_of_ST_ens__TbindP a b pre post
+      wp f (g : a -> ST.prog_tree b pre post)
+      (s_g : ST.shape_tree _ _ {forall (x : a) . ST.prog_has_shape (g x) s_g})
+      sl0 y sl1
+      (pre_eq_g  : (x : a) ->
+                   Lemma (req_equiv (g x) s_g sl0))
+      (post_eq_g : (x : a) ->
+                   Lemma (requires ST.tree_req (g x) sl0) (ensures ens_equiv (g x) s_g sl0 y sl1))
+  : Lemma
+      (requires ST.tree_req (ST.TbindP a b pre post wp f g) sl0)
+      (ensures  ens_equiv (ST.TbindP a b pre post wp f g) (SbindP _ _ s_g) sl0 y sl1)
+  =
+    let t = ST.TbindP a b pre post wp f g in
+    let s = SbindP _ _ s_g in
+    let r_g (x : a) = repr_Fun_of_ST (g x) s_g sl0 in
+    let post'g = post_Fun_of_ST post s_g in
+    let post'  = post_Fun_of_ST post s in
+    let sl1' : post_v post' y = sel_Fun_of_ST post s y sl1 in
+
+    assert (ens_equiv t s sl0 y sl1 == (
+      (as_requires wp /\
+      (exists (x : a) .
+        as_ensures wp x /\ ST.tree_ens (g x) sl0 y sl1)
+     <==>
+      (post_eq_src sl0 sl1 (post_src_of_shape s) /\
+      (as_requires wp /\
+      (exists (x : a) .
+       as_ensures wp x /\
+      (tree_req (r_g x) /\
+      (exists (yg : b) (sl1g : post_v (post_Fun_of_ST post #(L.length #Type pre) s_g) yg) .
+       tree_ens (r_g x) yg sl1g /\
+      (let sl1f = sel_ST_of_Fun (g x) s_g sl0 yg sl1g in
+       y == yg /\ sl1' == sel_Fun_of_ST post s yg sl1f
+      )))))))
+    )) by T.(trefl ());
+
+    assert (post_eq_src sl0 sl1 (post_src_of_shape s));
+
+    introduce forall (x : a {as_ensures wp x}) .
+      tree_req (r_g x) /\
+      (ST.tree_ens (g x) sl0 y sl1 <==>
+      (exists (sl1g : post_v post'g y) .
+         tree_ens (r_g x) y sl1g /\
+         sl1' == sel_Fun_of_ST post s y (sel_ST_of_Fun (g x) s_g sl0 y sl1g)))
+    with begin
+      U.assert_by (ST.tree_req (g x) sl0)
+        (fun () ->
+          let req_g x = ST.tree_req (g x) sl0 in
+          assert (ST.tree_req (ST.TbindP a b pre post wp f g) sl0 == (wp req_g /\ True))
+              by T.(trefl ());
+          U.prop_equal (fun p -> p) (ST.tree_req (ST.TbindP a b pre post wp f g) sl0) (wp req_g /\ True);
+          FStar.Monotonic.Pure.elim_pure_wp_monotonicity wp);
+      pre_eq_g x;
+
+      introduce forall (sl1g : post_v post'g y) .
+        sl1' == sel_Fun_of_ST post s y (sel_ST_of_Fun (g x) s_g sl0 y sl1g)
+        <==> (sl1g == sel_Fun_of_ST post s_g y sl1 /\
+            post_eq_src sl0 sl1 (post_src_of_shape s_g))
+       with begin
+        let sl1gST = sel_ST_of_Fun (g x) s_g sl0 y sl1g in
+         U.assert_by (sel_Fun_of_ST post s y sl1 == sel_Fun_of_ST post s y sl1gST
+                   ==> sl1 == sl1gST)
+          (fun () -> post_eq_src_ST_Fun_ST t s sl0 y sl1;
+                  post_eq_src_ST_Fun_ST t s sl0 y sl1gST);
+        sel_Fun_ST_Fun (g x) s_g sl0 y sl1g;
+        post_eq_src_iff (g x) s_g sl0 y sl1
+       end;
+       post_eq_g x
+    end
+
+
+#push-options "--z3rlimit 10"
+let rec repr_Fun_of_ST_req
+  (#a : Type u#a) (#pre : ST.pre_t u#b) (#post : ST.post_t u#a u#b a)
+  (t : ST.prog_tree a pre post) (s : ST.prog_shape t)
+  (sl0 : Dl.dlist pre)
+  : Lemma (ensures req_equiv t s sl0) (decreases t)
+  = ST.match_prog_tree t
+    (fun a pre post t -> (s : ST.prog_shape t) -> (sl0 : Dl.dlist pre) ->
+       squash (ST.tree_req t sl0 <==> tree_req (repr_Fun_of_ST t s sl0)))
+    (fun (*ST.Tequiv*) pre post0 p -> fun s sl0 -> ())
+    (fun (*ST.Tspec*) a pre post frame req ens -> fun s sl0 -> ())
+    (fun (*ST.Tret*) a x post -> fun s sl0 -> ())
+    begin fun (*ST.Tbind*) a b pre itm post f g -> fun s sl0 ->
+      let Sbind _ _ _ s_f s_g = s in
+      repr_Fun_of_ST_req f s_f sl0;
+      repr_Fun_of_ST_req__Tbind a b pre itm post f g s_f s_g sl0
+        (fun x sl1 -> repr_Fun_of_ST_req (g x) s_g sl1)
+        (fun x sl1 -> repr_Fun_of_ST_ens f s_f sl0 x sl1)
+    end
+    begin fun (*ST.TbindP*) a b pre post wp f g -> fun s sl0 ->
+      let SbindP _ _ s_g = s in
+      let pt0 x = ST.tree_req (g x) sl0 in
+      let pt1 x = tree_req (repr_Fun_of_ST (g x) s_g sl0) /\
+                    (forall (y : b) (sl1' : post_v (post_Fun_of_ST post #(L.length #Type pre) s_g) y) .
+                    tree_ens (repr_Fun_of_ST (g x) s_g sl0) y sl1' ==> True) in
+      calc (<==>) {
+        ST.tree_req (ST.TbindP a b pre post wp f g) sl0;
+      <==> { _ by T.(apply_lemma (`U.iff_refl); trefl ()) }
+        wp (fun x -> ST.tree_req (g x) sl0) /\ True;
+      <==> {}
+        wp pt0;
+      <==> { wp_morph_iff wp pt0 pt1 (fun x -> repr_Fun_of_ST_req (g x) s_g sl0) }
+        wp pt1;
+      <==> {}
+        wp (fun x -> tree_req (repr_Fun_of_ST (g x) s_g sl0) /\
+                (forall (y : b) (sl1' : post_v (post_Fun_of_ST post #(L.length #Type pre) s_g) y) .
+                tree_ens (repr_Fun_of_ST (g x) s_g sl0) y sl1' ==> True)) /\ True;
+      <==> { _ by T.(apply_lemma (`U.iff_refl); trefl ())}
+        tree_req (repr_Fun_of_ST (ST.TbindP a b pre post wp f g) (SbindP _ _ s_g) sl0);
+      }
+    end s sl0
+
+and repr_Fun_of_ST_ens
+  (#a : Type u#a) (#pre : ST.pre_t u#b) (#post : ST.post_t u#a u#b a)
+  (t : ST.prog_tree a pre post) (s : ST.prog_shape t)
+  (sl0 : Dl.dlist pre) (res : a) (sl1 : Dl.dlist (ST.post_ts post res))
+  : Lemma (requires  ST.tree_req t sl0)
+          (ensures   ens_equiv t s sl0 res sl1)
+          (decreases t)
+  = ST.match_prog_tree t
+    (fun a pre post t -> (s : ST.prog_shape t) ->
+       (sl0 : Dl.dlist pre) -> (res : a) -> (sl1 : Dl.dlist (ST.post_ts post res)) ->
+       squash (ST.tree_req t sl0) ->
+       squash (ens_equiv t s sl0 res sl1))
+    begin fun (*ST.Tequiv*) pre post0 p -> fun s sl0 Unit' sl1 () ->
+      introduce (forall (i : Fin.fin (L.length post0)) . Dl.index sl1 i === Dl.index sl0 (p i)) ==>
+                sl1 == Dl.apply_perm_r p sl0
+        with _ . Dl.dlist_extensionality sl1 (Dl.apply_perm_r p sl0) (fun _ -> ())
+    end
+    begin fun (*ST.Tspec*) a pre post frame req ens -> fun s sl0 x sl1 () ->
+      repr_Fun_of_ST_ens__Tspec a pre post frame req ens s sl0 x sl1
+    end
+    begin fun (*ST.Tret*) a x post -> fun s sl0 x sl1 () ->
+      post_Fun_of_ST__ret post;
+      Dl.dlist_extensionality (sel_Fun_of_ST post s x sl1) sl1 (fun _ -> ())
+    end
+    begin fun (*ST.Tbind*) a b pre itm post f g -> fun s sl0 y sl2 _ ->
+      let Sbind _ _ _ s_f s_g = s in
+      repr_Fun_of_ST_req f s_f sl0;
+      repr_Fun_of_ST_ens__Tbind a b pre itm post f g s_f s_g sl0 y sl2
+        (fun x sl1 -> repr_Fun_of_ST_req (g x) s_g sl1)
+        (fun x sl1 -> repr_Fun_of_ST_ens f s_f sl0 x sl1)
+        (fun x sl1 -> repr_Fun_of_ST_ens (g x) s_g sl1 y sl2)
+    end
+    begin fun (*ST.TbindP*) a b pre post wp f g -> fun s sl0 y sl1 _ ->
+      let SbindP _ _ s_g = s in
+      repr_Fun_of_ST_ens__TbindP a b pre post wp f g s_g sl0 y sl1
+        (fun x -> repr_Fun_of_ST_req (g x) s_g sl0)
+        (fun x -> repr_Fun_of_ST_ens (g x) s_g sl0 y sl1)
+    end s sl0 res sl1 ()
+#pop-options
+
+#pop-options
+
+
+
+(***** Test *)
+
+module Perm = Learn.Permutation
+module M = Experiment.Steel.Repr.M
+
+let test_ST : ST.prog_tree int [bool; int] (Lf.const int [bool; int])
+  = ST.(
+    b <-- Tspec bool [bool] (Lf.const bool [bool]) [int]
+           (fun _ -> True) (fun sl0 b sl1 -> Dl.index sl1 0 = Dl.index sl0 0 /\ b = Dl.index sl0 0);
+    Tequiv [bool; int] [int; bool] (Perm.perm_f_swap #2 0);;
+    x <-- Tspec int [int] (Lf.const int [int]) [bool]
+           (fun _ -> True) (fun sl0 x sl1 -> Dl.index sl1 0 = Dl.index sl0 0 /\ x = Dl.index sl0 0);
+    Tequiv [int; bool] [bool; int] (Perm.perm_f_swap #2 0);;
+    Tret int (if b then x else 0) (Lf.const int [bool; int])
+  )
+
+let test_ST_shape_tree : ST.shape_tree 2 2
+  = Sbind _ _ _ (Sspec  1 1 1)
+   (Sbind _ _ _ (Sequiv 2 (Perm.perm_f_swap #2 0))
+   (Sbind _ _ _ (Sspec  1 1 1)
+   (Sbind _ _ _ (Sequiv 2 (Perm.perm_f_swap #2 0))
+                (Sret   2))))
+
+let test_ST_has_shape () : squash (ST.prog_has_shape' test_ST test_ST_shape_tree)
+  = _ by T.(norm M.normal_spec_steps; norm [simplify]; smt ())
+
+let test_ST_shape : ST.prog_shape test_ST =
+  let _ = test_ST_has_shape () in test_ST_shape_tree
+
+let test_Fun (b_ini : bool) (x_ini : int) =
+  repr_Fun_of_ST test_ST test_ST_shape Dl.(DCons _ b_ini _ (DCons _ x_ini _ DNil))
+
+//let _ = fun b_ini x_ini ->
+//  assert (M.print_util (test_Fun b_ini x_ini))
+//    by T.(norm M.normal_spec_steps; qed ())
