pure/Learn.ListFun.fst
@@ -1,0 +1,102 @@
+module Learn.ListFun
+
+module U = Learn.Util
+module T = FStar.Tactics
+
+open FStar.List.Pure
+open Learn.List
+
+
+irreducible let __list_fun__ : unit = ()
+
+/// The type [list_fun a b] is isomorphic to [list (a -> b)].
+
+[@@ __list_fun__]
+noeq type list_fun (a b : Type) = {
+  lf_len  : nat;
+  lf_list : a -> (l : list b {length l = lf_len});
+}
+
+unfold
+let eta (#a #b : Type) (l : list_fun a b) : list_fun a b
+  = {
+    lf_len  = l.lf_len;
+    lf_list = U.eta l.lf_list
+  }
+
+let lf_eta_extensionality
+      (#a : Type) (#b : Type)
+      (f : list_fun a b) (g : list_fun a b {g.lf_len = f.lf_len})
+      (ef : squash (f == eta f)) (eg : squash (g == eta g))
+      (eq : (x:a -> i : nat {i < f.lf_len} -> Lemma (index (f.lf_list x) i == index (g.lf_list x) i)))
+  : Lemma (f == g)
+  = U.funext_eta (eta f).lf_list (eta g).lf_list (_ by T.(trefl ())) (_ by T.(trefl ()))
+                 (fun x -> list_extensionality (f.lf_list x) (g.lf_list x) (fun i -> eq x i))
+
+
+/// Conversions with [list (a -> b)]
+
+[@@ __list_fun__]
+let lf_of_list_f (#a #b : Type) (l : list (a -> b))
+                       (x : a)
+  : l' : list b {length l' = length l}
+  = map (U.app_on x b) l
+
+unfold
+let lf_of_list (#a #b : Type) (l : list (a -> b))
+  : list_fun a b
+  = {
+    lf_len  = length l;
+    lf_list = lf_of_list_f l
+  }
+
+[@@ __list_fun__]
+let lf_index (#a #b : Type) (l : list_fun a b)
+             (i : nat {i < l.lf_len}) (x : a)
+  : b
+  = index (l.lf_list x) i
+
+unfold
+let lf_to_list (#a #b : Type) (l : list_fun a b)
+  : list (a -> b)
+  = initi 0 l.lf_len (lf_index l)
+
+
+/// Operations
+
+unfold
+let const (a #b : Type) (l : list b)
+  : list_fun a b
+  = {
+    lf_len  = length l;
+    lf_list = U.const a #(l' : list b {length l' = length l}) l
+  }
+
+
+[@@ __list_fun__]
+let append_f #a #b (l0 l1 : list_fun a b) (x : a)
+  : l : list b {length l = l0.lf_len + l1.lf_len}
+  = (**) append_length (l0.lf_list x) (l1.lf_list x);
+    append (l0.lf_list x) (l1.lf_list x)
+
+unfold
+let append (#a #b : Type) (l0 l1 : list_fun a b)
+  : list_fun a b
+  = {
+    lf_len  = l0.lf_len + l1.lf_len;
+    lf_list = append_f l0 l1
+  }
+
+
+[@@ __list_fun__]
+let map_f #a #b #c (f : b -> c) (l : list_fun a b) (x : a)
+  : l' : list c {length l' = l.lf_len}
+  = map f (l.lf_list x)
+
+unfold
+let map #a #b #c (f : b -> c) (l : list_fun a b)
+  : list_fun a c
+  = {
+    lf_len  = l.lf_len;
+    lf_list = map_f f l
+  }
