pure/Learn.Option.fst
@@ -1,0 +1,6 @@
+module Learn.Option
+
+let bind #a #b (x : option a) (f : a -> option b) : option b
+  = match x with
+  | None   -> None
+  | Some x -> f x
